CaseStudies/TimedABP.thy
@@ -14,18 +14,35 @@ begin
 default_sort countable
 
 (* ----------------------------------------------------------------------- *)
-section {* Medium *}
+section {* components definition *}
 (* ----------------------------------------------------------------------- *)
 
 definition tsMed :: "'a tstream \<rightarrow> bool stream \<rightarrow> 'a tstream" where
 "tsMed \<equiv> \<Lambda> msg ora. tsProjFst\<cdot>(tsFilter {x. snd x}\<cdot>(tsZip\<cdot>msg\<cdot>ora))"
+
+definition tsRec :: "('a \<times> 'b) tstream \<rightarrow> ('b tstream \<times> 'a tstream)" where
+"tsRec \<equiv> \<Lambda> dat. (tsProjSnd\<cdot>dat, tsProjFst\<cdot>(tsRemDups\<cdot>dat))"
+
+(* ----------------------------------------------------------------------- *)
+section {* basic properties *}
+(* ----------------------------------------------------------------------- *)
+
+(* ----------------------------------------------------------------------- *)
+subsection {* medium *}
+(* ----------------------------------------------------------------------- *)
 
 (* Assumption for medium  lemmata: #({True} \<ominus> ora)=\<infinity> *)
 
 lemma tsmed_insert: "tsMed\<cdot>msg\<cdot>ora = tsProjFst\<cdot>(tsFilter {x. snd x}\<cdot>(tsZip\<cdot>msg\<cdot>ora))"
 by (simp add: tsMed_def)
 
-(* ToDo: Properties lemmata for medium *)
+(* ToDo: basic properties lemmata for medium *)
+
+lemma tsmed_strict [simp]: 
+  "tsMed\<cdot>\<bottom>\<cdot>\<epsilon> = \<bottom>"
+  "tsMed\<cdot>msg\<cdot>\<epsilon> = \<bottom>"
+  "tsMed\<cdot>\<bottom>\<cdot>ora = \<bottom>"
+oops
 
 (* Assumtions are missing. Add msg\<noteq>\<bottom> and ora\<noteq>\<bottom> as needed. *)
 lemma tsmed_mlscons_true: "tsMed\<cdot>(tsMLscons\<cdot>m\<cdot>msg)\<cdot>((updis True) && ora) = tsMLscons\<cdot>m\<cdot>(tsMed\<cdot>msg\<cdot>ora)"
@@ -36,18 +53,21 @@ oops
 
 lemma tsmed_delayfun: "ora \<noteq>\<bottom> \<Longrightarrow> tsMed\<cdot>(delayFun\<cdot>msg)\<cdot>ora = delayFun\<cdot>(tsMed\<cdot>msg\<cdot>ora)"
 oops
-
-text {* Not every message will be transmitted. *}    
-lemma tsmed_slen_leq:
-  shows "#(Rep_tstream (tsMed\<cdot>msg\<cdot>ora)) \<le> #(Rep_tstream msg)"
+ 
+text {* If infinite ticks will be sent infinite ticks will be transmitted. *}
+lemma tsmed_tstickcount [simp]: "#\<surd>(tsMed\<cdot>msg\<cdot>ora) = #\<surd>msg"
 oops
 
-text {* If infinity messages will be sent infinity messages will be transmitted. *}
+text {* Not every message will be transmitted. *}    
+lemma tsmed_slen_leq: "#(tsAbs\<cdot>(tsMed\<cdot>msg\<cdot>ora)) \<le> #(tsAbs\<cdot>msg)"
+oops
+
+text {* If infinite messages will be sent infinite messages will be transmitted. *}
 lemma tsmed_slen [simp]: assumes "#({True} \<ominus> ora)=\<infinity>" and "#(tsAbs\<cdot>msg)=\<infinity>" 
   shows "#(tsAbs\<cdot>(tsMed\<cdot>msg\<cdot>ora)) = \<infinity>"
 oops
 
-text {* If infinity ticks will be sent infinity ticks will be transmitted. *}
+text {* If just infinite ticks will be sent just infinite ticks will be transmitted. *}
 lemma tsmed_inftick [simp]: "#ora=\<infinity> \<Longrightarrow> tsMed\<cdot>tsInfTick\<cdot>ora = tsInfTick"
 oops
 
@@ -55,7 +75,11 @@ text {* Medium without oracle will transmit all messages and ticks. *}
 lemma tsmed_inftrue [simp]: "tsMed\<cdot>msg\<cdot>((\<up>True) \<infinity>) = msg"
 oops
 
-(* ToDo: More properties lemmata for medium, first show testings below *)
+(* ----------------------------------------------------------------------- *)
+section {* additional properties *}
+(* ----------------------------------------------------------------------- *)
+
+(* ToDo: additional properties lemmata for medium, first show testings below *)
 
 text {* Two medium can be reduced to one medium. *}
 lemma tsmed2med: obtains ora3 where "tsMed\<cdot>(tsMed\<cdot>msg\<cdot>ora1)\<cdot>ora2 = tsMed\<cdot>msg\<cdot>ora3"
@@ -69,23 +93,16 @@ oops
 
 lemma tsmed_map: "tsMed\<cdot>(tsMap f\<cdot>msg)\<cdot>ora = tsMap f\<cdot>(tsMed\<cdot>msg\<cdot>ora)"
 oops
-    
-(* ----------------------------------------------------------------------- *)
-section {* Receiver *}
-(* ----------------------------------------------------------------------- *)
-
-definition tsRec :: "('a \<times> 'b) tstream \<rightarrow> ('b tstream \<times> 'a tstream)" where
-"tsRec \<equiv> \<Lambda> dat. (tsProjSnd\<cdot>dat, tsProjFst\<cdot>(tsRemDups\<cdot>dat))"
 
 (* ----------------------------------------------------------------------- *)
 section {* Testing *}
 (* ----------------------------------------------------------------------- *)
 
+text {* equivalence classes: empty tstream, finite tstream, infinite tstream *}
+
 (* ----------------------------------------------------------------------- *)
 subsection {* Medium *}
 (* ----------------------------------------------------------------------- *)
-
-text {* equivalence classes: empty tstream, finite tstream, infinite tstream *}
 
 lift_definition OneTwoThree :: "nat tstream" is
   "<[Msg 1, \<surd>, Msg 2, \<surd>, Msg 3, \<surd>]>"
@@ -95,7 +112,7 @@ by (metis (no_types, lifting) assoc_sconc list2s.simps(1) list2s.simps(2) lscons
 lemma "tsMed\<cdot>\<bottom>\<cdot>((\<up>True) \<infinity>) = \<bottom>"
 by (simp add: tsmed_insert)
 
-(* ToDo: Testing lemmata *)
+(* ToDo: testing lemmata for medium *)
 
 lemma "tsMed\<cdot>OneTwoThree\<cdot>((\<up>True) \<infinity>) = OneTwoThree"
 oops
